src/SlowPrimeSynthesisExamples.v
@@ -87,7 +87,7 @@ Module debugging_sat_solinas_25519.
       let p := mul bound a b in
       let (lo, hi) := add_mul_limb' bound (firstn n p) (skipn n p) c 0 0 0 in
       if c * Z.abs hi <=? 2^machine_wordsize - c
-      then reduce' bound 1 c lo hi
+      then reduce' bound 1 c lo [hi]
       else lo ++ [hi].
 
     Goal True.
@@ -140,6 +140,19 @@ Module debugging_sat_solinas_25519.
                    (None, (None, tt))
                    (None)).
 
+    Fail Check ltac:(
+      let e := constr:(weight (fun _ => 10)%positive 2) in
+      let e := eval cbv [stream.map weight] in e in
+      (* let e := eval cbv delta [stream.prefixes] in e in *)
+      idtac e;
+      let r := Reify e in exact r).
+    Check ltac:(
+      let e := constr:(weight (fun _ => 10)%positive 2) in
+      let e := eval cbv [stream.map weight] in e in
+      let e := eval cbv delta [stream.prefixes] in e in
+      idtac e;
+      let r := Reify e in exact r).
+
     Time Redirect "log"
          Compute
          Show.show (* [show] for pretty-printing of the AST without needing lots of imports *)
@@ -149,34 +162,20 @@ Module debugging_sat_solinas_25519.
             false (* inline *)
             possible_values
             machine_wordsize
-            ltac:(let n := (eval cbv in n) (* needs to be reduced to reify correctly *) in
-                  let r := Reify (fun xs y => mulmod xs [y]) in
+            ltac:(let e := constr:(fun xs y =>
+                    let (lo, hi) := add_mul_limb' bound [] xs y 0 0 0 in
+                    reduce bound 1%nat 38 lo [hi]
+                  ) in
+                  let e := eval cbv delta [n reduce stream.map weight stream.prefixes] in e in
+                  let r := Reify e in
                   exact r)
                    (fun _ _ => []) (* comment *)
-                   (Some boundsn, (Some (r[0 ~>2^64-1]%zrange), tt))
+                   (Some boundsn, (Some (r[0 ~>2^58-1]%zrange), tt))
                    (Some boundsn)
                    (None, (None, tt))
                    (None)).
 
-    Time Redirect "log" Fail
-         Compute
-         Show.show (* [show] for pretty-printing of the AST without needing lots of imports *)
-         (Pipeline.BoundsPipelineToString
-            "fiat_" "fe4_canon"
-            false (* subst01 *)
-            false (* inline *)
-            possible_values
-            machine_wordsize
-            ltac:(let n := (eval cbv in n) (* needs to be reduced to reify correctly *) in
-            let r := Reify (canon bound (2^255-19)) in
-                  exact r)
-                   (fun _ _ => []) (* comment *)
-                   (Some boundsn, tt)
-                   (Some boundsn)
-                   (None, tt)
-                   (None)).
-
-    Goal (Z.to_nat (weight bound 4/(2^255-19))) = 2%nat. trivial. all: fail. Abort.
+    Goal (Z.to_nat (weight bound 4/(2^255-19))) = 2%nat. trivial. all: fail.
 
     Time Redirect "log"
          Compute
@@ -187,11 +186,9 @@ Module debugging_sat_solinas_25519.
             false (* inline *)
             possible_values
             machine_wordsize
-            ltac:(let n := (eval cbv in n) (* needs to be reduced to reify correctly *) in
-            let r := Reify (fun xs =>
-              dlet xs := condsub bound xs (encode bound 4 (2^255-19)) in
-              dlet xs := condsub bound xs (encode bound 4 (2^255-19)) in
-              xs) in
+            ltac:(let e := constr:(canon bound (2^255-19)) in
+                  let e := eval cbv delta [n canon stream.map weight stream.prefixes] in e in
+                  let r := Reify e in
                   exact r)
                    (fun _ _ => []) (* comment *)
                    (Some boundsn, tt)
